theories/iris/logrel/iris_fundamental_segfree.v
@@ -23,65 +23,116 @@ Section fundamental.
   (* --------------------------------------------------------------------------------------- *)
 
  
-(*  Lemma wss_select_nat a b a' b' tbs:
-    (a' >= a) -> (a' + b' <= a + b) -> length tbs = b ->
-    ↦[wss][ N.of_nat a ] tbs -∗
-      ∃ tbs', ⌜ (length tbs') = b' ⌝ ∗
-                                ↦[wss][ N.of_nat a' ] tbs' ∗
-                                (↦[wss][ N.of_nat a' ] tbs' -∗ ↦[wss][ N.of_nat a ] tbs).
-  Proof.
-    iIntros (Ha Hb Htbs) "Hs".
-    rewrite - (take_drop (a' - a) tbs).
-    rewrite - (take_drop b' (drop (a' - a) tbs)).
-    iDestruct (big_sepL_app with "Hs") as "[Hbegin Hs]".
-    iDestruct (big_sepL_app with "Hs") as "[Hs Hend]".
-    iExists (take b' (drop (a' - a) tbs)).
-    iSplit.
-    - iPureIntro. rewrite take_length_le; first done.
-      rewrite drop_length Htbs. lia.
-    - iSplitL "Hs".
-      + iApply (big_sepL_impl with "[Hs]"); first done.
-        iIntros "!>" (k x) "%Hx Hs".
-        rewrite take_length_le; last lia. repeat rewrite Nat2N.id.
-        replace (a + (a' - a + k)) with (a' + k); first done.
-        lia.
-      + iIntros "Hs".
-        iApply (big_sepL_app with "[$Hbegin Hs Hend]").
-        iApply (big_sepL_app with "[Hend Hs]").
-        iSplitL "Hs"; last done.
-        iApply (big_sepL_impl with "[Hs]"); first done.
-        iIntros "!>" (k x) "%Hx Hs".
-        rewrite take_length_le; last lia. repeat rewrite Nat2N.id.
-        replace (a + (a' - a + k)) with (a' + k); first done.
-        lia.
-  Qed.
-
-    Lemma wss_select a b a' b' tbs:
-    (a' >= a)%N -> (a' + b' <= a + b)%N -> N.of_nat (length tbs) = b ->
-    ↦[wss][ a ] tbs -∗
-      ∃ tbs', ⌜ N.of_nat (length tbs') = b' ⌝ ∗
-                                ↦[wss][ a' ] tbs' ∗
-                                (↦[wss][ a' ] tbs' -∗ ↦[wss][ a ] tbs).
-    Proof.
-      iIntros (Ha Hb Htbs) "Hs".
-      iDestruct (wss_select_nat (N.to_nat a) (N.to_nat b) (N.to_nat a') (N.to_nat b') tbs
-                  with "[Hs]") as "(%tbs' & % & ?)"; try lia.
-      - by rewrite N2Nat.id.
-      - repeat rewrite N2Nat.id. iExists tbs'. iFrame.
-        iPureIntro. lia.
-    Qed.  *)
-
-        
-                                                           
-    
-    
     
   (* ----------------------------------------- SEGFREE ---------------------------------------- *)
 
 
-  Lemma typing_segload C t : 
-    ⊢ semantic_typing C (to_e_list [BI_segfree t]) (Tf [T_handle] []).
+  Lemma typing_segfree C : 
+    ⊢ semantic_typing C (to_e_list [BI_segfree]) (Tf [T_handle] []).
   Proof.
+    unfold semantic_typing, interp_expression.
+    iIntros (i all lh hl).
+    iIntros "#Hi [%Hlh_base [%Hlh_len [%Hlh_valid #Hcont]]]" (f vs) "[Hf Hfv] #Hv".
+    iDestruct "Hv" as "[-> | Hv]".
+    { take_drop_app_rewrite_twice 0 1.
+      iApply (wp_wand _ _ _ (λ vs, ⌜vs = trapV⌝ ∗  ↪[frame]f)%I with "[Hf]").
+      { iApply (wp_trap with "[] [$]");auto. }
+      iIntros (v0) "[? ?]". iFrame. iExists _,_. iFrame "∗ #". }
+    iDestruct "Hv" as (ws ->) "Hv".
+    iDestruct (big_sepL2_length with "Hv") as %Hlen.
+    destruct ws as [|wh ws];[done|destruct ws; last done].  
+    iSimpl in "Hv". iDestruct "Hv" as "(Hv & _)".
+    rewrite fixpoint_interp_value_handle_eq.
+     iDestruct "Hv" as (h) "(-> & [%Hval | (%γ & %base' & %bound' & #Hw & %Hbase & %Hbound & #Hinv)])".
+    { iApply (wp_wand with "[Hf]").
+        - iApply (wp_segfree_failure_1 with "[$Hf]"). 
+          + by right.
+          + by instantiate (1 := λ x, ⌜ x = trapV ⌝%I).
+        - iIntros (v) "[-> Hf]".
+          iSplitR; first by do 2 iLeft.
+          iExists _, _. iFrame. } 
+
+
+
+    destruct (valid h) eqn:Hvalid.
+    2: { iApply (wp_wand with "[Hf]").
+        - iApply (wp_segfree_failure_1 with "[$Hf]"). 
+          + by right.
+          + by instantiate (1 := λ x, ⌜ x = trapV ⌝%I).
+        - iIntros (v) "[-> Hf]".
+          iSplitR; first by do 2 iLeft.
+          iExists _, _. iFrame. }
+
+    destruct (offset h =? 0)%N eqn:Hoff.
+    2:{ apply N.eqb_neq in Hoff. iApply (wp_wand with "[Hf]").
+      - iApply (wp_segfree_failure_1 with "[$Hf]"). 
+        + by left.
+        + by instantiate (1 := λ x, ⌜ x = trapV ⌝%I).
+      - iIntros (v) "[-> Hf]".
+        iSplitR; first by do 2 iLeft.
+        iExists _, _. iFrame. }
+    apply N.eqb_eq in Hoff.
+
+    
+    
+    iDestruct "Hfv" as "[(%fall & Hbl & Htoks) Hfv]".
+    iDestruct (gamma_agree with "Hw Hbl") as "%Hγ".
+    rewrite - (insert_delete _ _ _ Hγ).
+    iDestruct (big_sepM_insert with "Htoks") as "[(%Hx & Ha & Hown) Htoks]";
+      first by rewrite lookup_delete.
+    iApply fupd_wp. Check ghost_map_delete.  Search (ghost_map_auth _ _ (delete _ _)).
+    unfold gamma_id_white.
+    Search (_ ↪[_]□ _ -∗ _ ↪[_] _)%I.
+    iMod (ghost_map_delete with "Hbl [Hw]").
+    { unfold gamma_id_white. iExact "Hw".
+    destruct (base' =? base h)%N eqn:Hnbase.
+    2:{ apply N.eqb_neq in Hnbase. iApply (wp_wand with "[Hf Ha]").
+        - iApply (wp_segfree_failure_2 with "[$Hf $Ha]") => //; try by left.
+          iNext. iIntros "Ha". instantiate (1 := λ x, (⌜ x = trapV ⌝ ∗ _)%I).
+          iSplit; first done. iExact "Ha".
+        - iIntros (v) "[[-> Ha] Hf]".
+          iSplitR; first by do 2 iLeft.
+          iExists _, _. iFrame.
+          iExists _. iFrame. admit.  (*rewrite insert_delete => //. 
+          iDestruct (big_sepM_insert. iApply "Htoks". iFrame. done. *)
+    }
+(*    destruct (n0 =? bound h)%N eqn:Hnbound.
+    2:{ apply N.eqb_neq in Hnbound. iApply (wp_wand with "[Hf Ha]").
+        - iApply (wp_segfree_failure_2 with "[$Hf $Ha]") => //; try by right.
+          iNext. iIntros "Ha". instantiate (1 := λ x, (⌜ x = trapV ⌝ ∗ _)%I).
+          iSplit; first done. iExact "Ha".
+        - iIntros (v) "[[-> Ha] Hf]".
+          iSplitR; first by do 2 iLeft.
+          iExists _, _. iFrame.
+          iExists _. iFrame. iApply "Htoks". iExists _. iFrame. done.
+    } *)
+    iSimpl.
+    apply N.eqb_eq in Hnbase as ->.
+(*    apply N.eqb_eq in Hnbound as ->. *)
+    iApply fupd_wp. 
+    iMod (cinv_cancel with "Hinv Hown") as "(%tbs & >%Htbs & >Hss & #Hhandles)"; first solve_ndisj.
+      iDestruct (wss_select (N.to_nat (base h)) (N.to_nat bound') (N.to_nat (handle_addr h)) (N.to_nat bound') tbs with "[Hss]") 
+        as "(%Htbs' & Hss & Hreconstitute)";
+        try rewrite N2Nat.id;
+        try done;
+        try by subst; unfold handle_addr; lia.
+      unfold handle_addr. rewrite Hoff N.add_0_r.
+      unfold handle_addr in Htbs'. rewrite Hoff N.add_0_r in Htbs'. 
+    iModIntro.
+    iApply (wp_wand with "[Hf Ha Hss]").
+    { iApply (wp_wand with "[Hf Ha Hss]").
+      - iApply (wp_segfree with "[$Hf $Hss $Ha]") => //.
+        by instantiate (1 := λ x, ⌜ x = immV [] ⌝%I).
+      - iIntros (v) "[-> Hf]". instantiate (1 := λ x, (⌜ x = immV [] ⌝ ∗ ↪[frame] f)%I).
+        by iFrame. }
+    iIntros (v) "[-> Hf]".
+    iSplitR.
+    - iLeft; iRight. iExists _. iSplit => //. 
+    - iExists _,_. iFrame. iExists _. iFrame "Htoks".
+      Search "ghost_map_del".
+      admit.
+      
+    
   Admitted. 
 (*    unfold semantic_typing, interp_expression.
     iIntros (i all lh hl).
