theories/iris/logrel/iris_fundamental_segstore.v
@@ -22,89 +22,174 @@ Section fundamental.
   (* -------------------------------------- EXPRESSIONS ------------------------------------ *)
   (* --------------------------------------------------------------------------------------- *)
 
- 
-(*  Lemma wss_select_nat a b a' b' tbs:
-    (a' >= a) -> (a' + b' <= a + b) -> length tbs = b ->
-    ↦[wss][ N.of_nat a ] tbs -∗
-      ∃ tbs', ⌜ (length tbs') = b' ⌝ ∗
-                                ↦[wss][ N.of_nat a' ] tbs' ∗
-                                (↦[wss][ N.of_nat a' ] tbs' -∗ ↦[wss][ N.of_nat a ] tbs).
+  
+  Lemma lookup_map {A B} (f: A -> B) l k:
+    map f l !! k = match l !! k with Some x => Some (f x) | None => None end.
   Proof.
-    iIntros (Ha Hb Htbs) "Hs".
-    rewrite - (take_drop (a' - a) tbs).
-    rewrite - (take_drop b' (drop (a' - a) tbs)).
-    iDestruct (big_sepL_app with "Hs") as "[Hbegin Hs]".
-    iDestruct (big_sepL_app with "Hs") as "[Hs Hend]".
-    iExists (take b' (drop (a' - a) tbs)).
-    iSplit.
-    - iPureIntro. rewrite take_length_le; first done.
-      rewrite drop_length Htbs. lia.
-    - iSplitL "Hs".
-      + iApply (big_sepL_impl with "[Hs]"); first done.
-        iIntros "!>" (k x) "%Hx Hs".
-        rewrite take_length_le; last lia. repeat rewrite Nat2N.id.
-        replace (a + (a' - a + k)) with (a' + k); first done.
-        lia.
-      + iIntros "Hs".
-        iApply (big_sepL_app with "[$Hbegin Hs Hend]").
-        iApply (big_sepL_app with "[Hend Hs]").
-        iSplitL "Hs"; last done.
-        iApply (big_sepL_impl with "[Hs]"); first done.
-        iIntros "!>" (k x) "%Hx Hs".
-        rewrite take_length_le; last lia. repeat rewrite Nat2N.id.
-        replace (a + (a' - a + k)) with (a' + k); first done.
-        lia.
+    generalize dependent k.
+    induction l => //=; intros.
+    destruct k => //=.
+  Qed. 
+  
+
+  Lemma take_drop_take {A} lo hi lo' (l: list A) :
+    lo + hi <= lo' ->
+    take hi (drop lo (take lo' l)) = take hi (drop lo l).
+  Proof.
+    intros H. generalize dependent lo'; generalize dependent hi; generalize dependent lo.
+    induction l => //=; intros.
+    { rewrite take_nil drop_nil take_nil. done. }
+    destruct hi => //=.
+    destruct lo' => //=; first lia.
+    destruct lo => //=.
+    { specialize (IHl 0). rewrite drop_0 in IHl. erewrite <- IHl.
+      - rewrite drop_0. rewrite take_take.
+        replace (hi `min` lo') with hi; last lia.
+        rewrite take_take.
+        instantiate (1 := lo').
+        replace (hi `min` lo') with hi; last lia.
+        done.
+      - lia. }
+    rewrite IHl; last lia. done.
   Qed.
 
-    Lemma wss_select a b a' b' tbs:
-    (a' >= a)%N -> (a' + b' <= a + b)%N -> N.of_nat (length tbs) = b ->
-    ↦[wss][ a ] tbs -∗
-      ∃ tbs', ⌜ N.of_nat (length tbs') = b' ⌝ ∗
-                                ↦[wss][ a' ] tbs' ∗
-                                (↦[wss][ a' ] tbs' -∗ ↦[wss][ a ] tbs).
-    Proof.
-      iIntros (Ha Hb Htbs) "Hs".
-      iDestruct (wss_select_nat (N.to_nat a) (N.to_nat b) (N.to_nat a') (N.to_nat b') tbs
-                  with "[Hs]") as "(%tbs' & % & ?)"; try lia.
-      - by rewrite N2Nat.id.
-      - repeat rewrite N2Nat.id. iExists tbs'. iFrame.
-        iPureIntro. lia.
-    Qed.  *)
-
-        
-                                                           
-    
-    
-    
-  (* ----------------------------------------- SEGSTORE ---------------------------------------- *)
-
-
-  Lemma typing_segload C t : 
-    ⊢ semantic_typing C (to_e_list [BI_segstore t]) (Tf [t; T_handle] []).
+  Lemma overlap_nat a b a' b':
+    a + S b > a' -> a' + S b' > a -> exists x, a <= x /\ x < a + S b /\ a' <= x /\ x < a' + S b'.
   Proof.
-  Admitted. 
-(*    unfold semantic_typing, interp_expression.
-    iIntros (i all lh hl).
+    intros H H'.
+    induction b.
+    { exists a. repeat split; lia. }
+    destruct (a + S b =? a') eqn:Ha.
+    { apply Nat.eqb_eq in Ha.
+      exists a'. repeat split; lia. }
+    apply Nat.eqb_neq in Ha.
+    assert (a + S b > a') as Ha'.
+    { lia. }
+    apply IHb in Ha' as (x & ? & ? & ? & ?).
+    exists x. repeat split; lia. 
+  Qed.
+
+  Lemma overlap a b a' b':
+    (b > 0 -> b' > 0 ->
+     a + b > a' -> a' + b' > a -> exists x, a <= x /\ x < a + b /\ a' <= x /\ x < a' + b')%N.
+  Proof.
+    intros Hb Hb' H H'.
+    destruct (overlap_nat (N.to_nat a) ((N.to_nat b - 1)) (N.to_nat a') ((N.to_nat b' - 1))) as (x & ? & ? & ? & ?); try lia.
+    exists (N.of_nat x). repeat split; lia.
+  Qed.
+
+  Lemma lookup_lt_Some_inv {A} i (l: list A):
+    i < length l -> exists x, l !! i = Some x.
+  Proof.
+    generalize dependent i.
+    induction l; intros; first by simpl in *; lia.
+    destruct i; first by eexists a.
+    simpl in H. assert (i < length l) as Hi; first lia.
+    apply IHl in Hi as [x Hx].
+    exists x. simpl. done.
+  Qed. 
+
+
+  Lemma modulo_divisible a m:
+    (a `mod` m = 0 -> (a / m) * m = a)%N.
+  Proof.
+    unfold N.modulo, N.div.
+    specialize (N.div_eucl_spec a m) as H. 
+    destruct (N.div_eucl a m) eqn:Hdivmod.
+    simpl.
+    intros ->.
+    lia.
+  Qed. 
+    
+
+  
+  Lemma modulo_trapped a b m :
+    (a `mod` m = 0 -> b `mod` m = 0 -> a > b - m -> a < b + m -> a = b)%N.
+  Proof.
+    intros Ha Hb Hlo Hhi.
+    apply modulo_divisible in Ha, Hb => //.
+    remember (a `div` m)%N as ka; clear Heqka.
+    remember (b `div` m)%N as kb; clear Heqkb.
+    remember (N.to_nat a) as a'.
+    remember (N.to_nat b) as b'.
+    remember (N.to_nat m) as m'.
+    remember (N.to_nat ka) as ka'.
+    remember (N.to_nat kb) as kb'.
+    assert (ka' * m' = a') as Ha'; first lia.
+    assert (kb' * m' = b') as Hb'; first lia.
+    assert (a' > b' - m') as Hlo'; first lia.
+    assert (a' < b' + m') as Hhi'; first lia.
+    assert (a' = b'); last lia.
+    assert (b' - a' = (kb' - ka') * m') as Hamb.
+    { rewrite - Ha' - Hb'. 
+      rewrite Nat.mul_sub_distr_r.
+      done. }
+    remember (kb' - ka') as k; clear Heqk.
+    assert (b' - a' < m'); first lia.
+    destruct k; last lia. 
+    assert (b' <= a'); first lia.
+    assert (a' - b' = (ka' - kb') * m') as Hbma.
+    { rewrite - Ha' - Hb'. 
+      rewrite Nat.mul_sub_distr_r.
+      done. }
+     remember (ka' - kb') as k; clear Heqk.
+     assert (a' - b' < m'); first lia.
+     destruct k; last lia.
+     lia.
+  Qed.
+
+  Lemma modulo_leq a m:
+    (a `mod` m = 0 -> a = 0 \/ a >= m)%N.
+  Proof.
+    intro H; apply modulo_divisible in H.
+    remember (a `div` m)%N as k; clear Heqk.
+    remember (N.to_nat a) as a'.
+    remember (N.to_nat m) as m'.
+    remember (N.to_nat k) as k'.
+    assert (k' * m' = a') as H'; first lia.
+    assert (a' = 0 \/ a' >= m') as [?|?]; [|lia|lia].
+    destruct k'; first by left.
+    right; lia.
+  Qed. 
+    
+    
+
+    
+    (* ----------------------------------------- SEGSTORE ---------------------------------------- *)
+
+
+  Lemma typing_segstore_numeric C t :
+    t <> T_handle ->
+    ⊢ semantic_typing C (to_e_list [BI_segstore t]) (Tf [T_handle; t] []).
+  Proof.
+    unfold semantic_typing, interp_expression.
+    iIntros (Ht i all lh hl).
     iIntros "#Hi [%Hlh_base [%Hlh_len [%Hlh_valid #Hcont]]]" (f vs) "[Hf Hfv] #Hv".
     iDestruct "Hv" as "[-> | Hv]".
     { take_drop_app_rewrite_twice 0 1.
       iApply (wp_wand _ _ _ (λ vs, ⌜vs = trapV⌝ ∗  ↪[frame]f)%I with "[Hf]").
       { iApply (wp_trap with "[] [$]");auto. }
-      iIntros (v0) "[? ?]". iFrame. iExists _. iFrame "∗ #". }
+      iIntros (v0) "[? ?]". iFrame. iExists _,_. iFrame "∗ #". }
     iDestruct "Hv" as (ws ->) "Hv".
     iDestruct (big_sepL2_length with "Hv") as %Hlen.
-    destruct ws as [|w ws];[done|destruct ws;[|done]].
-    iSimpl in "Hv". iDestruct "Hv" as "[Hv _]".
+    destruct ws as [|wh ws];[done|destruct ws as [|w ws];[done|destruct ws;[|done]]].
+    iSimpl in "Hv". iDestruct "Hv" as "(Hvh & Hv & _)".
     rewrite fixpoint_interp_value_handle_eq.
-    iDestruct "Hv" as (h γ base' bound') "(-> & #Hw & %Hbase & %Hbound & #Hinv)".
+    iDestruct (interp_value_agree with "Hv") as "%Hagree".
 
+    iDestruct "Hvh" as (h) "(-> & [%Hval | (%γ & %base' & %bound' & #Hw & %Hbase & %Hbound & #Hinv)])".
+    { iApply (wp_wand with "[Hf]").
+      - iApply (wp_segstore_failure with "[$Hf]"); first done.
+        + by left.
+        + by instantiate (1 := λ x, ⌜ x = trapV ⌝%I).
+      - iIntros (v) "[-> Hf]".
+        iSplitR; first by do 2 iLeft.
+        iExists _. iFrame. } 
     iSimpl.
-
-
 
     destruct (valid h) eqn:Hvalid.
     2:{ iApply (wp_wand with "[Hf]").
-        - iApply (wp_segload_failure with "[$Hf]").
+        - iApply (wp_segstore_failure with "[$Hf]"); first done.
           + by left.
           + by instantiate (1 := λ x, ⌜ x = trapV ⌝%I).
         - iIntros (v) "[-> Hf]".
@@ -114,7 +199,7 @@ Section fundamental.
     destruct (bound h <? offset h + N.of_nat (t_length t))%N eqn:Hbounds.
     { apply N.ltb_lt in Hbounds.
       iApply (wp_wand with "[Hf]").
-      - iApply (wp_segload_failure with "[$Hf]").
+      - iApply (wp_segstore_failure with "[$Hf]"); first done.
         + by right; left; lia.
         + by instantiate (1 := λ x, ⌜ x = trapV ⌝%I).
       - iIntros (v) "[-> Hf]".
@@ -122,52 +207,344 @@ Section fundamental.
           iExists _. iFrame. } 
     apply N.ltb_ge in Hbounds.
 
-    iDestruct "Hfv" as "[Halloc Hfv]".
-    iDestruct "Halloc" as (γmap) "[Hbl Htok]".
-    iApply fupd_wp. 
-    iDestruct "Hfv" as (locs Hlocs) "[#Hlocs Hown]".
-    iDestruct (gamma_agree with "Hw Hbl") as "%Hid".
-    iDestruct (big_sepM_lookup_acc _ _ _ _ Hid with "Htok") as "[(%x & %Hx & Halloc & Htok) Htoks]".
-    iMod (cinv_acc with "Hinv Htok") as "(Hss & Hwon & Hcls)"; first solve_ndisj.
-    iDestruct "Hss" as (tbs) "(>%Htbs & >Hss & Hhandles)".
-    iDestruct (wss_select base' bound' (handle_addr h) (N.of_nat (t_length t)) tbs with "Hss")
-      as "(%tbs' & %Htbs' & Hss & Hreconstitute)"; try by subst; unfold handle_addr; lia.
-    assert (length tbs' = t_length t) as Htbs''; first lia. 
 
-    destruct t eqn:Ht.
+    iApply (wp_wand _ _ _ (λ x, (⌜ x = immV [] ⌝ ∗ interp_frame (tc_local C) i all f) ∗ ↪[frame] f )%I with "[Hf Hfv]").
+    { iApply (wp_atomic _ _ (⊤ ∖ ↑(wsN (id h)))).
+      iDestruct "Hfv" as "[Halloc Hfv]".
+      iDestruct "Halloc" as (γmap) "[Hbl Htok]".
+      iDestruct "Hfv" as (locs Hlocs) "[#Hlocs Hown]".
+      iDestruct (gamma_agree with "Hw Hbl") as "%Hid".
+      iDestruct (big_sepM_lookup_acc _ _ _ _ Hid with "Htok") as "[(%x & %Hx & Halloc & Htok) Htoks]".
+      iMod (cinv_acc with "Hinv Htok") as "(Hss & Hwon & Hcls)"; first solve_ndisj.
+      iModIntro.
+      iDestruct "Hss" as (tbs) "(>%Htbs & >Hss & #Hhandles)".
+      iDestruct (wss_select (N.to_nat base') (N.to_nat bound') (N.to_nat (handle_addr h)) (t_length t) tbs with "[Hss]") 
+        as "(%Htbs' & Hss & Hreconstitute)";
+        try rewrite N2Nat.id;
+        try done;
+        try by subst; unfold handle_addr; lia.
+      remember (take (t_length t) (drop (N.to_nat (handle_addr h) - N.to_nat base') tbs)) as tbs'.
+      
+      assert (length tbs' = t_length t) as Htbs''; first lia. 
 
-    - (* Segload T_i32 *)
-      iApply (wp_wand _ _ _ (λ vs, (⌜ vs = immV _ ⌝ ∗ _) ∗ _)%I with "[Hf Halloc Hss]"). 
-      + iApply (wp_segload_deserialize with "[$Hf $Halloc $Hss]") => //.
-      + iIntro (v) "(-> & Halloc & Hss)". iMod ("Hcls" with "[Hss Hhandles]"). iIntros (v).
-    
-    destruct (N_lt_dec (mem_length ms) ((Wasm_int.N_of_uint i32m z) + off + (N.of_nat (t_length t))))%N.
-      { iApply wp_fupd.
-        iApply (wp_wand _ _ _ (λ vs, (⌜vs = trapV⌝ ∗ _) ∗ _)%I with "[Hsize Hf]").
-        { by iApply (wp_load_failure with "[$Hf $Hsize]");[by rewrite Hlocs /=|by apply N.lt_gt|]. }
-        iIntros (v) "[[-> Hsize] Hf]".
-        iMod ("Hcls" with "[$Hown Hsize Hmem]") as "Hown".
-        { iNext. iExists _. iFrame. }
-        iModIntro.
-        iSplitR;[by iLeft; iLeft|iExists _;iFrame].
-        iExists _. eauto. 
-      }
-      { iDestruct (mem_extract _ (Wasm_int.N_of_uint i32m z + off) (t_length t) with "Hmem") as (bv) "[Ha [Hmem %Hlenbv]]";[destruct t;simpl;try lia; try apply hsnz|lia|].
-        iApply wp_fupd.
-        iApply (wp_wand _ _ _ (λ vs, (⌜vs = immV _⌝ ∗ _) ∗ _)%I with "[Ha Hf]").
-        { iApply (wp_load_deserialize with "[$Hf $Ha]");eauto;by rewrite Hlocs /=. }
-        iIntros (v) "[[-> Ha] Hf]".
-        iDestruct ("Hmem" with "Ha") as "Hmem".
-        iMod ("Hcls" with "[$Hown Hsize Hmem]") as "Hown".
-        { iNext. iExists _. iFrame. }
-        iModIntro.
-        iSplitR;[iLeft; iRight|iExists _;iFrame;iExists _;eauto].
-        iExists _. iSplit;[eauto|]. iSimpl.
-        iSplit =>//. unfold interp_value.
-        destruct t;iSimpl;eauto.
-      }
-
+      iApply (wp_wand _ _ _ (λ v, ((|={⊤ ∖ ↑wsN (id h),⊤}=>
+                                       (⌜v = immV []⌝ ∗ interp_frame (tc_local C) i all f)) ∗  ↪[frame]f))%I
+                 with "[Hf Hbl Hown Halloc Htoks Hwon Hcls Hss Hreconstitute]").
+        2:{ iIntros (v) "[H Hf]". iFrame. } 
+        iApply wp_segstore => //.
+        iSplitR "Halloc Hss Hf"; last by iFrame.
+        iNext. iIntros "(Hid & Hss)".
+        assert (length (map (λ b, (b, Numeric)) (bits w)) = t_length t) as Hlen'.
+        { rewrite map_length. by apply length_bits. } 
+        iDestruct ("Hreconstitute" $! _ Hlen' with "Hss") as "Hss".
+        rewrite N2Nat.id.
+        iMod ("Hcls" with "[Hss]").
+        + iNext. iExists _. iFrame "Hss". iSplit.
+          * iPureIntro. repeat rewrite app_length.
+            rewrite drop_length Hlen' take_length_le.
+            2:{ rewrite Htbs. unfold handle_addr. lia. }
+            unfold handle_addr. lia.
+          * (* We must now restore the invariant on all stored handles to be valid *)
+            iIntros (addr) "%Haddr".
+            (* We must show that knowning addr is handle-aligned, it either doesn't store
+               a handle, or stores a valid one *)
+            destruct (handle_addr h - base' + N.of_nat (t_length t) <=? addr)%N eqn:Hlo.
+              
+            -- (* Case 1: the place where we wrote to memory is before addr *)
+              (* I.e. the previous invariant still holds *)
+              apply N.leb_le in Hlo.
+               iDestruct ("Hhandles" $! addr Haddr) as "[%Hnum | Hvalid]";
+                 destruct Haddr as [Hmod Haddr].
+               ++ iLeft. 
+                  iPureIntro.
+                  destruct Hnum as (addr' & b & Haddr' & Hnum).
+                  exists addr', b. split; first done.
+                  rewrite lookup_app.
+                  rewrite lookup_take_ge; last lia.
+                  rewrite lookup_app.
+                  rewrite lookup_ge_None_2.
+                  2:{ rewrite map_length take_length_le; try lia.
+                      erewrite length_bits => //. lia. }
+                  rewrite lookup_drop.
+                  rewrite map_length take_length_le; try lia.
+                  erewrite length_bits => //.
+                  replace  (N.to_nat (handle_addr h) - N.to_nat base' + t_length t +
+                              (N.to_nat (addr + addr') - (N.to_nat (handle_addr h) - N.to_nat base') -
+                                 t_length t)) with (N.to_nat (addr + addr')); first done.
+                  lia.
+               ++ iRight.
+                  rewrite catA.
+                  rewrite drop_app_ge.
+                  2:{ rewrite app_length map_length take_length_le; try lia.
+                      erewrite length_bits => //. lia. } 
+                  rewrite drop_drop.
+                  rewrite app_length map_length take_length_le; last lia.
+                  erewrite length_bits => //.
+                  rewrite - le_plus_minus; last lia.
+                  done.
+            -- apply N.leb_gt in Hlo.
+               destruct (addr + handle_size <=? handle_addr h - base')%N eqn:Hhi.
+               ++ (* Case 2: the place where we wrote is far after addr *)
+               (* i.e. the previous invariant still holds *)
+                 apply N.leb_le in Hhi.
+                  iDestruct ("Hhandles" $! addr Haddr) as "[%Hnum | Hvalid]";
+                    destruct Haddr as [Hmod Haddr].
+                 ** iLeft. 
+                    iPureIntro.
+                    destruct Hnum as (addr' & b & Haddr' & Hnum).
+                    exists addr', b. split; first done.
+                    rewrite lookup_app.
+                    rewrite lookup_take; last lia.
+                    rewrite Hnum. done.
+                 ** iRight. 
+                    rewrite drop_app_le.
+                    2:{ rewrite take_length. lia. }
+                    
+                    rewrite take_app_le.
+                    2:{ rewrite drop_length take_length. lia. }
+                    rewrite take_drop_take => //.
+                    lia.
+                
+               ++ (* Case 3: the place where we wrote is right after addr *)
+                 (* I.e. we know that a handle isn't stored there -- we just wrote
+                    a numerical value *)
+                 apply N.leb_gt in Hhi.
+                 iLeft.
+                 iPureIntro. specialize hsnz as Hsize. rewrite nat_bin in Hsize.
+                 destruct (overlap addr handle_size (handle_addr h - base') (N.of_nat (t_length t))) as (y & ? & ? & ? & ?); try lia; try by destruct t.
+                 assert (N.to_nat (addr + (y - addr)) - (N.to_nat (handle_addr h) - N.to_nat base') < length (bits w)) as Hbits.
+                 { erewrite length_bits => //. lia. }
+                 apply lookup_lt_Some_inv in Hbits as [b Hb].
+                 exists (y - addr)%N, b.
+                 split; first lia.
+                 rewrite lookup_app.
+                 rewrite lookup_take_ge; last lia.
+                 rewrite cat_app.
+                 rewrite lookup_app.
+                 rewrite take_length_le; last lia.
+                 rewrite lookup_map. rewrite Hb. done.
+        + iModIntro. 
+          iSplitR => //.
+          iSplitR "Hown".
+          -- iExists _. iFrame. iApply ("Htoks" with "[Hwon Hid]").
+               iExists _. iFrame. done.
+          -- iExists _. iFrame. iSplit; done.
     }
-  Qed. *)
+    iIntros (v) "[(-> & Hfv) Hf]".
+    iSplitR.
+      + iLeft. iRight. iExists _. iSplit; first done. done. 
+      + iExists _. iFrame.
+  Qed.
+
+  
+  Lemma typing_segstore C t :
+    ⊢ semantic_typing C (to_e_list [BI_segstore t]) (Tf [T_handle; t] []).
+  Proof.
+    destruct t; try by apply typing_segstore_numeric.
+    unfold semantic_typing, interp_expression.
+    iIntros (i all lh hl).
+    iIntros "#Hi [%Hlh_base [%Hlh_len [%Hlh_valid #Hcont]]]" (f vs) "[Hf Hfv] #Hv".
+    iDestruct "Hv" as "[-> | Hv]".
+    { take_drop_app_rewrite_twice 0 1.
+      iApply (wp_wand _ _ _ (λ vs, ⌜vs = trapV⌝ ∗  ↪[frame]f)%I with "[Hf]").
+      { iApply (wp_trap with "[] [$]");auto. }
+      iIntros (v0) "[? ?]". iFrame. iExists _. iFrame "∗ #". }
+    iDestruct "Hv" as (ws ->) "Hv".
+    iDestruct (big_sepL2_length with "Hv") as %Hlen.
+    destruct ws as [|wh ws];[done|destruct ws as [|w ws];[done|destruct ws;[|done]]].
+    iSimpl in "Hv". iDestruct "Hv" as "(Hvh & Hv & _)".
+    do 2 rewrite fixpoint_interp_value_handle_eq.
+    iDestruct "Hv" as (hv) "[-> Hv]".
+
+    iDestruct "Hvh" as (h) "(-> & [%Hval | (%γ & %base' & %bound' & #Hw & %Hbase & %Hbound & #Hinv)])".
+    { iApply (wp_wand with "[Hf]").
+      - iApply (wp_segstore_failure with "[$Hf]"); first done.
+        + by left.
+        + by instantiate (1 := λ x, ⌜ x = trapV ⌝%I).
+      - iIntros (v) "[-> Hf]".
+        iSplitR; first by do 2 iLeft.
+        iExists _. iFrame. } 
+    iSimpl.
+
+    destruct (valid h) eqn:Hvalid.
+    2:{ iApply (wp_wand with "[Hf]").
+        - iApply (wp_segstore_failure with "[$Hf]"); first done.
+          + by left.
+          + by instantiate (1 := λ x, ⌜ x = trapV ⌝%I).
+        - iIntros (v) "[-> Hf]".
+          iSplitR; first by do 2 iLeft.
+          iExists _. iFrame. } 
+
+    destruct (bound h <? offset h + N.of_nat (t_length T_handle))%N eqn:Hbounds.
+    { apply N.ltb_lt in Hbounds.
+      iApply (wp_wand with "[Hf]").
+      - iApply (wp_segstore_failure with "[$Hf]"); first done.
+        + by right; left; lia.
+        + by instantiate (1 := λ x, ⌜ x = trapV ⌝%I).
+      - iIntros (v) "[-> Hf]".
+          iSplitR; first by do 2 iLeft.
+          iExists _. iFrame. } 
+    apply N.ltb_ge in Hbounds.
+
+    destruct ((handle_addr h `mod` handle_size)%N =? N.of_nat 0)%N eqn:Hmod.
+    2:{  iApply (wp_wand with "[Hf]").
+         - iApply (wp_segstore_failure with "[$Hf]") => //.
+           + right; right; split => //. intros Habs.
+             rewrite Habs in Hmod. simpl in Hmod. done.
+           + by instantiate (1 := λ x, ⌜ x = trapV ⌝%I).
+         - iIntros (v) "[-> Hf]".
+           iSplitR; first by do 2 iLeft.
+           iExists _. iFrame. } 
+    apply N.eqb_eq in Hmod.
+
+    assert (types_agree T_handle (VAL_handle hv)) as Hagree; first done.
+
+    iApply (wp_wand _ _ _ (λ x, (⌜ x = immV [] ⌝ ∗ interp_frame (tc_local C) i all f) ∗ ↪[frame] f )%I with "[Hf Hfv]").
+    { iApply (wp_atomic _ _ (⊤ ∖ ↑(wsN (id h)))).
+      iDestruct "Hfv" as "[Halloc Hfv]".
+      iDestruct "Halloc" as (γmap) "[Hbl Htok]".
+      iDestruct "Hfv" as (locs Hlocs) "[#Hlocs Hown]".
+      iDestruct (gamma_agree with "Hw Hbl") as "%Hid".
+      iDestruct (big_sepM_lookup_acc _ _ _ _ Hid with "Htok") as "[(%x & %Hx & Halloc & Htok) Htoks]".
+      iMod (cinv_acc with "Hinv Htok") as "(Hss & Hwon & Hcls)"; first solve_ndisj.
+      iModIntro.
+      iDestruct "Hss" as (tbs) "(>%Htbs & >Hss & #Hhandles)".
+      iDestruct (wss_select (N.to_nat base') (N.to_nat bound') (N.to_nat (handle_addr h)) (t_length T_handle) tbs with "[Hss]") 
+        as "(%Htbs' & Hss & Hreconstitute)";
+        try rewrite N2Nat.id;
+        try done;
+        try by subst; unfold handle_addr; lia.
+      remember (take (t_length T_handle) (drop (N.to_nat (handle_addr h) - N.to_nat base') tbs)) as tbs'.
+      
+      assert (length tbs' = t_length T_handle) as Htbs''; first lia. 
+
+      iApply (wp_wand _ _ _ (λ v, ((|={⊤ ∖ ↑wsN (id h),⊤}=>
+                                       (⌜v = immV []⌝ ∗ interp_frame (tc_local C) i all f)) ∗  ↪[frame]f))%I
+                 with "[Hf Hbl Hown Halloc Htoks Hwon Hcls Hss Hreconstitute]").
+        2:{ iIntros (v) "[H Hf]". iFrame. } 
+        iApply wp_segstore_handle => //; try by unfold t_length; rewrite nat_bin; lia.
+        iSplitR "Halloc Hss Hf"; last by iFrame.
+        iNext. iIntros "(Hid & Hss)".
+        assert (length (map (λ b, (b, Handle)) (bits (VAL_handle hv))) = t_length T_handle) as Hlen'.
+        { rewrite map_length. by apply length_bits. } 
+        iDestruct ("Hreconstitute" $! _ Hlen' with "Hss") as "Hss".
+        rewrite N2Nat.id.
+        iMod ("Hcls" with "[Hss]").
+        + iNext. iExists _. iFrame "Hss". iSplit.
+          * iPureIntro. repeat rewrite app_length.
+            rewrite drop_length Hlen' take_length_le.
+            2:{ rewrite Htbs. unfold handle_addr. lia. }
+            unfold handle_addr. lia.
+          * (* We must now restore the invariant on all stored handles to be valid *)
+            iIntros (addr) "%Haddr".
+            (* We must show that knowning addr is handle-aligned, it either doesn't store
+               a handle, or stores a valid one *)
+(*            destruct (handle_addr h + handle_size <=? base' + addr)%N eqn:Hlo. *)
+            destruct (handle_addr h - base' + N.of_nat (t_length T_handle) <=? addr)%N eqn:Hlo. 
+              
+            -- (* Case 1: the place where we wrote to memory is before addr *)
+              (* I.e. the previous invariant still holds *)
+              apply N.leb_le in Hlo.
+              iDestruct ("Hhandles" $! addr Haddr) as "[%Hnum | Hvalid]";
+                 destruct Haddr as [Hmod' Haddr].
+               ++ iLeft. 
+                  iPureIntro.
+                  destruct Hnum as (addr' & b & Haddr' & Hnum).
+                  exists addr', b. split; first done.
+                  rewrite lookup_app.
+                  rewrite lookup_take_ge; last lia.
+                  rewrite lookup_app.
+                  rewrite lookup_ge_None_2.
+                  2:{ rewrite map_length take_length_le; try lia.
+                      erewrite length_bits => //. lia. 
+                  }
+                  rewrite lookup_drop.
+                  rewrite map_length take_length_le; try lia.
+                  erewrite length_bits => //.
+                  replace  (N.to_nat (handle_addr h) - N.to_nat base' + t_length T_handle +
+                              (N.to_nat (addr + addr') - (N.to_nat (handle_addr h) - N.to_nat base') -
+                                 t_length T_handle)) with (N.to_nat (addr + addr')); first done.
+                  lia.
+               ++ iRight.
+                  rewrite catA.
+                  rewrite drop_app_ge.
+                  2:{ rewrite app_length map_length take_length_le; try lia.
+                      erewrite length_bits => //. lia. } 
+                  rewrite drop_drop.
+                  rewrite app_length map_length take_length_le; last lia.
+                  erewrite length_bits => //.
+                  rewrite - le_plus_minus; last lia.
+                  done.
+            -- apply N.leb_gt in Hlo.
+               destruct (addr + handle_size <=? handle_addr h - base')%N eqn:Hhi.
+               ++ (* Case 2: the place where we wrote is far after addr *)
+               (* i.e. the previous invariant still holds *)
+                 apply N.leb_le in Hhi.
+                  iDestruct ("Hhandles" $! addr Haddr) as "[%Hnum | Hvalid]";
+                    destruct Haddr as [Hmod' Haddr].
+                 ** iLeft. 
+                    iPureIntro.
+                    destruct Hnum as (addr' & b & Haddr' & Hnum).
+                    exists addr', b. split; first done.
+                    rewrite lookup_app.
+                    rewrite lookup_take; last lia.
+                    rewrite Hnum. done.
+                 ** iRight. 
+                    rewrite drop_app_le.
+                    2:{ rewrite take_length. lia. }
+                    
+                    rewrite take_app_le.
+                    2:{ rewrite drop_length take_length. lia. }
+                    rewrite take_drop_take => //.
+                    lia.
+                
+               ++ (* Case 3: the place where we wrote is right after addr *)
+                 (* I.e. we know that this handle is safe as it is our argument *)
+
+                 apply N.leb_gt in Hhi.
+                 iRight.
+                 destruct Haddr as [Hmod' Haddr].
+                 unfold t_length in Hlo. rewrite nat_bin N2Nat.id in Hlo.
+                 assert (handle_addr h < base' + addr + handle_size)%N as Hhi'; first lia.
+                 assert (handle_addr h > base' + addr - handle_size)%N as Hlo'.
+                 { lia. specialize (modulo_leq _ _ Hmod') as [Hz | Hsize].
+                   - rewrite Hz. 
+
+                   2:{ lia.
+                                 admit. } 
+                 
+                 specialize (modulo_trapped _ _ _ Hmod Hmod' Hlo' Hhi') as Heqaddr.
+                 assert (N.to_nat addr = length (take (N.to_nat (handle_addr h) - N.to_nat base') tbs)) as Hlentake.
+                 { rewrite take_length_le; last lia. lia. } 
+                 rewrite Hlentake drop_app.
+                 assert (N.to_nat handle_size = length (map (λ b, (b, Handle)) (bits (VAL_handle hv)))) as Hlenmap.
+                 { rewrite map_length. erewrite length_bits => //. unfold t_length.
+                   by rewrite nat_bin. }
+                 rewrite Hlenmap take_app.
+                 unfold bits. rewrite map_map.
+                 rewrite map_id.
+                 assert (handle_of_bytes (serialise_handle hv) = hv) as ->.
+                 { destruct HHB.
+                   unfold handle.handle_of_bytes, handle.serialise_handle.
+                   rewrite handle_of_serialise. done. } 
+                 rewrite fixpoint_interp_value_handle_eq.
+                 iExists hv. iSplit; first done.
+                 rewrite map_length.
+                 assert (length (serialise_handle hv) = N.to_nat handle_size) as ->.
+                 { destruct HHB. unfold handle.serialise_handle, handle.handle_size.
+                   rewrite length_serialise nat_bin. done. }
+                 iExact "Hv". 
+        + iModIntro. 
+          iSplitR; first done.
+          iSplitR "Hown".
+            -- iExists _. iFrame. iApply ("Htoks" with "[Hwon Hid]").
+               iExists _. iFrame. done.
+            -- iExists _. iFrame. iSplit; done.
+    }
+    iIntros (v) "[( -> & Hfv) Hf]".
+    iSplitR.
+      + iLeft. iRight. iExists _. iSplit; first done. done. 
+      + iExists _. iFrame.
+Qed.
 
 End fundamental.
