theories/segment_list.v
@@ -92,7 +92,7 @@ Fixpoint find_and_remove (nid : N) (l: list (N * N * N)) : option (list (N * N *
 
 Definition find_address nid l :=
   match find_and_remove nid l.(allocated) with
-  | Some (_,a, n) => Some (a,n)
+  | Some (_,a, n) => Some (a)
   | None => None end. 
 
 
